Format code
Signed-off-by: Anand Krishnamoorthi <anakrish@microsoft.com>

Rego.Interpreter.fst
@@ -4,87 +4,89 @@
 module Rego.Interpreter
 
 open Rego.Ast
+
 open Rego.Value
 
-type intr=interpreter
+type intr = interpreter
 
-let make_new () = {
-   rules = [];
-   scopes = [];
-   loop_exprs = [];
-}
+let make_new () = { rules = []; scopes = []; loop_exprs = [] }
 
 type loop_iteration = {
-  loop_expr: Ast.expr;
-  loop_value: value;
-  bindings: list (string & value)
+  loop_expr:Ast.expr;
+  loop_value:value;
+  bindings:list (string & value)
 }
 
 let iresult a = intr -> a & intr
-let (let!) #a #b (f:iresult a) (g:a -> iresult b) : iresult b = fun i -> let (a', i') = f i in g a' i'
-let return #a (x:a) : iresult a = fun i -> (x, i)
+
+let ( let! ) #a #b (f: iresult a) (g: (a -> iresult b)) : iresult b =
+  fun i ->
+    let a', i' = f i in
+    g a' i'
+
+let return #a (x: a) : iresult a = fun i -> (x, i)
+
 let get () : iresult intr = fun i -> (i, i)
+
 let set i : iresult unit = fun _ -> ((), i)
-let run #a (f:iresult a) (i:intr) : a & intr = f i
 
-let lookup_loop_expr (e:expr) : iresult _ = 
-  let! i = get() in
-  return <| List.Tot.find (fun (k,_) -> k = e) i.loop_exprs
+let run #a (f: iresult a) (i: intr) : a & intr = f i
 
-let rec lookup_var_in_scopes (scopes:list scope) (name:string) =
-    match scopes with
-    | hd::tl ->
-      (match List.Tot.find (fun (n,_) -> n = name) hd with
+let lookup_loop_expr (e: expr) : iresult _ =
+  let! i = get () in
+  return <| List.Tot.find (fun (k, _) -> k = e) i.loop_exprs
+
+let rec lookup_var_in_scopes (scopes: list scope) (name: string) =
+  match scopes with
+  | hd :: tl ->
+    (match List.Tot.find (fun (n, _) -> n = name) hd with
       | Some (_, v) -> v
       | None -> lookup_var_in_scopes tl name)
-    | _ -> Undefined
+  | _ -> Undefined
 
-let lookup_local_var (name:string) : iresult value =
-    let! i = get () in
-    return <| lookup_var_in_scopes i.scopes name
+let lookup_local_var (name: string) : iresult value =
+  let! i = get () in
+  return <| lookup_var_in_scopes i.scopes name
 
-let rec make_array_loop_iterations col (le:expr) (idx:string) (idxv:nat)
-: Tot (list loop_iteration)
-= 
-match col with
-| [] -> []
-| hd::tl ->
-  let itr = match idx with
-    | "_" -> { loop_expr=le; loop_value=hd; bindings = [] }
-    | _ -> { loop_expr=le; loop_value=hd; bindings = [(idx, Number idxv)] }
-  in
-    itr::make_array_loop_iterations tl le idx (idxv + 1)
+let rec make_array_loop_iterations col (le: expr) (idx: string) (idxv: nat)
+    : Tot (list loop_iteration) =
+  match col with
+  | [] -> []
+  | hd :: tl ->
+    let itr =
+      match idx with
+      | "_" -> { loop_expr = le; loop_value = hd; bindings = [] }
+      | _ -> { loop_expr = le; loop_value = hd; bindings = [(idx, Number idxv)] }
+    in
+    itr :: make_array_loop_iterations tl le idx (idxv + 1)
 
-let rec make_set_loop_iterations col (le:expr) (idx:string)
-: Tot (list loop_iteration)
-= 
-match col with
-| [] -> []
-| hd::tl ->
-  let itr = match idx with
-    | "_" -> { loop_expr=le; loop_value=hd; bindings = [] }
-    | _ -> { loop_expr=le; loop_value=hd; bindings = [(idx, hd)] }
-  in
-    itr::make_set_loop_iterations tl le idx
+let rec make_set_loop_iterations col (le: expr) (idx: string) : Tot (list loop_iteration) =
+  match col with
+  | [] -> []
+  | hd :: tl ->
+    let itr =
+      match idx with
+      | "_" -> { loop_expr = le; loop_value = hd; bindings = [] }
+      | _ -> { loop_expr = le; loop_value = hd; bindings = [(idx, hd)] }
+    in
+    itr :: make_set_loop_iterations tl le idx
 
-let rec make_object_loop_iterations col (le:expr) (idx:string)
-: Tot (list loop_iteration)
-= 
-match col with
-| [] -> []
-| (k,v)::tl ->
-  let itr = match idx with
-    | "_" -> { loop_expr=le; loop_value=v; bindings = [] }
-    | _ -> { loop_expr=le; loop_value=v; bindings = [(idx, k)] }
-  in
-    itr::make_object_loop_iterations tl le idx
+let rec make_object_loop_iterations col (le: expr) (idx: string) : Tot (list loop_iteration) =
+  match col with
+  | [] -> []
+  | (k, v) :: tl ->
+    let itr =
+      match idx with
+      | "_" -> { loop_expr = le; loop_value = v; bindings = [] }
+      | _ -> { loop_expr = le; loop_value = v; bindings = [(idx, k)] }
+    in
+    itr :: make_object_loop_iterations tl le idx
 
-
-let rec hoist_loops_in_expr (e:expr) (loops:list expr) 
-: iresult(list expr)
-= match e with
-  (* TODO: should we avoid hoisting if the index var is already defined? *)
-  | RefBrack (refr, Var _) -> hoist_loops_in_expr refr (e::loops)
+let rec hoist_loops_in_expr (e: expr) (loops: list expr) : iresult (list expr) =
+  match e with
+  | RefBrack (refr, Var _) ->
+    (* TODO: should we avoid hoisting if the index var is already defined? *)
+    hoist_loops_in_expr refr (e :: loops)
   | RefBrack (refr, _) -> hoist_loops_in_expr refr loops
   | Ast.Array arr -> hoist_loops_in_exprs arr loops
   | Ast.Set set -> hoist_loops_in_exprs set loops
@@ -94,66 +96,60 @@ let rec hoist_loops_in_expr (e:expr) (loops:list expr)
   | RefDot (refr, _) -> hoist_loops_in_expr refr loops
   | BinExpr (_, lhs, rhs)
   | BoolExpr (_, lhs, rhs)
-  | ArithExpr (_, lhs, rhs) 
-  | AssignExpr (_, lhs, rhs) -> 
+  | ArithExpr (_, lhs, rhs)
+  | AssignExpr (_, lhs, rhs) ->
     let! lps = hoist_loops_in_expr lhs loops in
     hoist_loops_in_expr rhs lps
   | MembershipExpr (k, v, c) ->
     let! lps1 = hoist_loops_in_expr k loops in
     let! lps2 = hoist_loops_in_expr v lps1 in
     hoist_loops_in_expr c lps2
-  | ArrayCompr _ | SetCompr _ | ObjectCompr _  -> return loops
-  | Var _ | Value _  -> return loops
+  | ArrayCompr _ | SetCompr _ | ObjectCompr _ -> return loops
+  | Var _ | Value _ -> return loops
 
-and hoist_loops_in_exprs exprs loops
-: iresult (list expr)
-= match exprs with
+and hoist_loops_in_exprs exprs loops : iresult (list expr) =
+  match exprs with
   | [] -> return loops
-  | hd::tl -> 
+  | hd :: tl ->
     let! lps = hoist_loops_in_expr hd loops in
     hoist_loops_in_exprs tl lps
 
-and hoist_loops_in_fields fields loops
-: iresult (list expr)
-= match fields with
+and hoist_loops_in_fields fields loops : iresult (list expr) =
+  match fields with
   | [] -> return loops
-  | (k, v)::tl -> 
+  | (k, v) :: tl ->
     let! lps1 = hoist_loops_in_expr k loops in
     let! lps2 = hoist_loops_in_expr v lps1 in
     hoist_loops_in_fields tl lps2
 
-let rec hoist_loops_in_stmts stmts : iresult (list literalStmt)
-= match stmts with
-| [] -> return []
-| hd::tl -> 
-  let! tl' = hoist_loops_in_stmts tl in
-  match hd.literal with
-  | Expr e -> 
-    let! exprs = hoist_loops_in_expr e [] in
-    let loops = List.Tot.map (fun e -> { literal = LoopExpr e; with_mods = []}) exprs in
-    let pfx = List.Tot.append loops [hd] in
-    return <| List.Tot.append pfx tl'
-  | _ -> return <| List.Tot.append [hd] tl' 
+let rec hoist_loops_in_stmts stmts : iresult (list literalStmt) =
+  match stmts with
+  | [] -> return []
+  | hd :: tl ->
+    let! tl' = hoist_loops_in_stmts tl in
+    match hd.literal with
+    | Expr e ->
+      let! exprs = hoist_loops_in_expr e [] in
+      let loops = List.Tot.map (fun e -> { literal = LoopExpr e; with_mods = [] }) exprs in
+      let pfx = List.Tot.append loops [hd] in
+      return <| List.Tot.append pfx tl'
+    | _ -> return <| List.Tot.append [hd] tl'
 
+let hoist_loops_in_query q : iresult query =
+  let! stmts = hoist_loops_in_stmts q.stmts in
+  return ({ stmts = stmts })
 
-let hoist_loops_in_query q : iresult query
-= let! stmts = hoist_loops_in_stmts q.stmts in
-  return { stmts = stmts }
+let lookup_var (ident: string) : iresult value = lookup_local_var ident
 
-let lookup_var (ident:string)
-: iresult value
-= lookup_local_var ident
-
-let rec eval_expr (e:expr)
-: iresult value
-= match! lookup_loop_expr e with
-  | Some((_, v)) -> return v
+let rec eval_expr (e: expr) : iresult value =
+  match! lookup_loop_expr e with
+  | Some (_, v) -> return v
   | None ->
     match e with
     | Var v -> lookup_var v
     | Value v -> return v
     | Ast.Array elems -> eval_array_elems elems []
-    | Ast.Set elems -> eval_set_elems elems [] 
+    | Ast.Set elems -> eval_set_elems elems []
     | Ast.Object fields -> eval_fields fields (Object [])
     | Ast.ArrayCompr query -> eval_query_stmts query.stmts (Value.Array [])
     | Ast.SetCompr query -> eval_query_stmts query.stmts (Value.Set [])
@@ -163,29 +159,26 @@ let rec eval_expr (e:expr)
     | Ast.AssignExpr olr -> eval_assign_expr olr
     | _ -> return Undefined
 
-and eval_array_elems (elems:list expr) (values:list value)
-: iresult value
-= match elems with
+and eval_array_elems (elems: list expr) (values: list value) : iresult value =
+  match elems with
   | [] -> return <| Value.Array (List.Tot.rev values)
-  | hd::tl ->
+  | hd :: tl ->
     match! eval_expr hd with
     | Undefined -> return Undefined
-    | v -> eval_array_elems tl (v::values)
+    | v -> eval_array_elems tl (v :: values)
 
-and eval_set_elems (elems:list expr) (values:list value)
-: iresult value
-= match elems with
+and eval_set_elems (elems: list expr) (values: list value) : iresult value =
+  match elems with
   | [] -> return <| List.Tot.fold_left Value.insert_into_set (Value.Set []) values
-  | hd::tl ->
+  | hd :: tl ->
     match! eval_expr hd with
     | Undefined -> return Undefined
-    | v -> eval_set_elems tl (v::values)
+    | v -> eval_set_elems tl (v :: values)
 
-and eval_fields (fields:list (expr*expr)) (obj:value)
-: iresult value
-= match fields with
+and eval_fields (fields: list (expr * expr)) (obj: value) : iresult value =
+  match fields with
   | [] -> return obj
-  | (key_expr,value_expr)::tl ->
+  | (key_expr, value_expr) :: tl ->
     match! eval_expr key_expr with
     | Undefined -> return Undefined
     | kv ->
@@ -194,8 +187,8 @@ and eval_fields (fields:list (expr*expr)) (obj:value)
       | vv -> eval_fields tl (insert_into_object obj kv vv)
 
 
-and eval_stmts_in_loop (iterations:list loop_iteration) (stmts:list literalStmt) (out:value)
-: Tot (iresult value) (decreases %[stmts; 1; iterations])
+and eval_stmts_in_loop (iterations: list loop_iteration) (stmts: list literalStmt) (out: value)
+    : Tot (iresult value) (decreases %[stmts;1;iterations]) =
   (* what decreases is the lexicographic ordering of the list of statements and the list of loop expressions, in that order;
      however, we also make a recursive call to an auxiliary eval_query_stmts, and that explains the additional '1' in the order, 
      i.e., we can call the auxiliary function with the same stmts, so long as that aux function doesn't
@@ -203,106 +196,101 @@ and eval_stmts_in_loop (iterations:list loop_iteration) (stmts:list literalStmt)
 
      See the "trick" mentioned in the note here: https://fstar-lang.org/tutorial/book/part1/part1_termination.html#mutual-recursion
       *)
-= 
-match iterations with
-| [] -> return out
-| hd::tl -> 
-  let! orig_i = get() in
-  set { orig_i with loop_exprs = (hd.loop_expr, hd.loop_value)::orig_i.loop_exprs;
-       scopes=hd.bindings::orig_i.scopes};!
-  let! out1 = eval_query_stmts stmts out in
-  set orig_i ;!
-  eval_stmts_in_loop tl stmts out1
-
-and eval_stmt stmt (out:value) 
-: iresult (value&value)
-= match stmt.literal with
-    | ArrayComprOutput e ->
-      let! v = eval_expr e in
-      return <| (Bool true, insert_into_array out v)
-    | SetComprOutput e ->
-      let! v = eval_expr e in
-      return <| (Bool true, insert_into_set out v)
-    | ObjectComprOutput (ke, ve) ->
-      let! kv = eval_expr ke in
-      let! vv = eval_expr ve in
-      return <| (Bool true, insert_into_object out kv vv)
-    | Expr e -> 
-      let! v = eval_expr e in
-      return <| (v, out)
-    | _ -> 
-      return (Undefined, Undefined)
-
-
-and eval_query_stmts (stmts:list literalStmt) (out:value)
-  : Tot(iresult value) (decreases %[stmts;0])
-= match stmts with
+  match iterations with
   | [] -> return out
-  | hd::tl ->
+  | hd :: tl ->
+    let! orig_i = get () in
+    let! _ =
+      set ({
+            orig_i with
+            loop_exprs = (hd.loop_expr, hd.loop_value) :: orig_i.loop_exprs;
+            scopes = hd.bindings :: orig_i.scopes
+          })
+    in
+    let! out1 = eval_query_stmts stmts out in
+    let! _ = set orig_i in
+    eval_stmts_in_loop tl stmts out1
+
+and eval_stmt stmt (out: value) : iresult (value & value) =
+  match stmt.literal with
+  | ArrayComprOutput e ->
+    let! v = eval_expr e in
+    return <| (Bool true, insert_into_array out v)
+  | SetComprOutput e ->
+    let! v = eval_expr e in
+    return <| (Bool true, insert_into_set out v)
+  | ObjectComprOutput (ke, ve) ->
+    let! kv = eval_expr ke in
+    let! vv = eval_expr ve in
+    return <| (Bool true, insert_into_object out kv vv)
+  | Expr e ->
+    let! v = eval_expr e in
+    return <| (v, out)
+  | _ -> return (Undefined, Undefined)
+
+
+and eval_query_stmts (stmts: list literalStmt) (out: value)
+    : Tot (iresult value) (decreases %[stmts;0]) =
+  match stmts with
+  | [] -> return out
+  | hd :: tl ->
     match hd.literal with
     | LoopExpr le ->
-      let! iterations = match le with
-      | RefBrack (refr, Var index) ->
-        let! col = eval_expr refr in
-        (match col with
-        | Array arr -> return <| make_array_loop_iterations arr le index 0
-        | Set set -> return <| make_set_loop_iterations set le index
-        | Object fields -> return <| make_object_loop_iterations fields le index
-        | _ -> return [])
-      | _ -> return []
-      in eval_stmts_in_loop iterations tl out
+      let! iterations =
+        match le with
+        | RefBrack (refr, Var index) ->
+          let! col = eval_expr refr in
+          (match col with
+            | Array arr -> return <| make_array_loop_iterations arr le index 0
+            | Set set -> return <| make_set_loop_iterations set le index
+            | Object fields -> return <| make_object_loop_iterations fields le index
+            | _ -> return [])
+        | _ -> return []
+      in
+      eval_stmts_in_loop iterations tl out
     | _ ->
-      let! (v, out') = eval_stmt hd out in
+      let! v, out' = eval_stmt hd out in
       match v with
       | Bool false | Undefined -> return Undefined
       | _ -> eval_query_stmts tl out'
-  
+
 (* todo chaining *)
-and eval_ref_dot rf
-: iresult value
-= let refr, field = rf in
+and eval_ref_dot rf : iresult value =
+  let refr, field = rf in
   let! v = eval_expr refr in
   return <| lookup_path v [Value.String field]
 
 (* todo chaining *)
-and eval_ref_brack (pr:expr*expr)
-: Tot (iresult value)
-= let refr, index = pr in
+and eval_ref_brack (pr: expr * expr) : Tot (iresult value) =
+  let refr, index = pr in
   let! v = eval_expr refr in
   let! idx = eval_expr index in
-  return <| lookup_path v (idx::[])
+  return <| lookup_path v ([idx])
 
 (* todo...actual implementation is quite complex *)
-and eval_assign_expr (t: (assignOp*expr*expr))
-: iresult value
-= let (_, lhs, rhs) = t in
+and eval_assign_expr (t: (assignOp * expr * expr)) : iresult value =
+  let _, lhs, rhs = t in
   match lhs with
-  | Var name -> (
-    let! rv = eval_expr rhs in
-    match rv with
-    | Undefined ->
-      return Undefined
-    | _ -> (* todo check existing binding *)
-      let! i = get() in
-      match i.scopes with
-      | hd::tl -> 
-        set {i with scopes = ((name, rv)::hd)::tl};!
-        return <| Bool true
-      | _ -> 
-        return Undefined
-    )
-  | _ ->
-    return Undefined
+  | Var name ->
+    (let! rv = eval_expr rhs in
+      match rv with
+      | Undefined -> return Undefined
+      | _ ->
+        (* todo check existing binding *)
+        let! i = get () in
+        match i.scopes with
+        | hd :: tl ->
+          let! _ = set ({ i with scopes = ((name, rv) :: hd) :: tl }) in
+          return <| Bool true
+        | _ -> return Undefined)
+  | _ -> return Undefined
 
-let eval (i:intr) (e:Ast.expr) : (value*intr) =
-  run (eval_expr e) i
+let eval (i: intr) (e: Ast.expr) : (value * intr) = run (eval_expr e) i
 
-let eval_user_query' (q:Ast.query)
-: iresult value
-= let! i = get() in
-  set { i with scopes = []::i.scopes } ;!
+let eval_user_query' (q: Ast.query) : iresult value =
+  let! i = get () in
+  let! _ = set ({ i with scopes = [] :: i.scopes }) in
   let! q1 = hoist_loops_in_query q in
   eval_query_stmts q1.stmts (Value.Array [])
 
-let eval_user_query (i:intr) (q:Ast.query) : (value*intr) =
-  run (eval_user_query' q) i
+let eval_user_query (i: intr) (q: Ast.query) : (value * intr) = run (eval_user_query' q) i
