Rego.Interpreter.fsti
@@ -2,14 +2,16 @@
 // Licensed under the MIT License.
 
 module Rego.Interpreter
+
 open Rego.Ast
+
 open Rego.Value
 
-type scope = list (string*value)
+type scope = list (string * value)
 
 type array_compr_ctx = {
-  ac_output_expr: expr;
-  ac_value: value
+  ac_output_expr:expr;
+  ac_value:value
 }
 
 type context =
@@ -18,13 +20,13 @@ type context =
 
 noeq
 type interpreter = {
-  rules: list (string*rule);
-  scopes: list scope;
-  loop_exprs: list (expr*value);
+  rules:list (string * rule);
+  scopes:list scope;
+  loop_exprs:list (expr * value)
 }
 
-val make_new () : interpreter
+val make_new (_: unit) : interpreter
 
-val eval (i:interpreter) (e:expr) : (value*interpreter)
+val eval (i: interpreter) (e: expr) : (value * interpreter)
 
-val eval_user_query (i:interpreter) (q:query) : (value*interpreter)
+val eval_user_query (i: interpreter) (q: query) : (value * interpreter)
