Rego.Main.fst
@@ -4,35 +4,42 @@
 module Rego.Main
 
 open Rego.Ast
+
 open Rego.Interpreter
+
 open Rego.Value
 
+let v1 = insert_at_path (Object []) ([String "hello"; String "world"]) (Number 42)
 
-let v1 = insert_at_path (Object []) (String "hello"::String "world"::[]) (Number 42)
-let v2 = insert_at_path v1 (String "monde"::[]) v1
-let v3 = insert_at_path v2 (v2::[]) v2
-let v4 = Array (v1::v2::v3::[])
+let v2 = insert_at_path v1 ([String "monde"]) v1
 
-let expr = Ast.Array (
-  Ast.Value (String "hello")::
-  Ast.Value (String "world")::
-  Ast.Array (
-    Ast.Value (Number 42)::
-    Ast.Set (
-      Ast.Value (Number 3)::
-      Ast.Value (Number 2)::
-      Ast.Value (Number 1)::
-      Ast.Object (
-        (Ast.Value (String "Hello"), Ast.Value (String "World"))
-        ::[]
-      )::
-      []
-    )::[]
-  )::[]
-)
+let v3 = insert_at_path v2 ([v2]) v2
 
-let intr = Interpreter.make_new()
-let (v5, intr1) = Interpreter.eval intr expr
+let v4 = Array ([v1; v2; v3])
+
+let expr =
+  Ast.Array
+  ([
+      Ast.Value (String "hello");
+      Ast.Value (String "world");
+      Ast.Array
+      ([
+          Ast.Value (Number 42);
+          Ast.Set
+          ([
+              Ast.Value (Number 3);
+              Ast.Value (Number 2);
+              Ast.Value (Number 1);
+              Ast.Object ([(Ast.Value (String "Hello"), Ast.Value (String "World"))])
+            ])
+        ])
+    ])
+
+let intr = Interpreter.make_new ()
+
+let v5, intr1 = Interpreter.eval intr expr
+
+
 
 // [ [e, f, g] |
 //  true
@@ -44,79 +51,64 @@ let (v5, intr1) = Interpreter.eval intr expr
 // ]
 // Produces:
 // [ ["Hello", 0, "English"], ["Salut", 0, "French"], [41, 1, 0], [47, 1, 1]]
-let query = {
-  stmts= [
-    { literal = Expr(Value(Bool true)); with_mods=[]; }; // true
-    { literal =
-       Expr(AssignExpr
-             (ColEq,
-              (Var "a"),
-              (Ast.Object [
+
+let query =
+  {
+    stmts
+    =
+    [
+      // true
+      { literal = Expr (Value (Bool true)); with_mods = [] };
+      {
+        literal
+        =
+        Expr
+        (AssignExpr
+          (ColEq,
+            (Var "a"),
+            (Ast.Object
+              [
                 (Value (String "English"), Value (String "Hello"));
-                (Value (String "French"), Value (String "Salut"));
-               ]))
-       );
-       with_mods=[];
-    };
-    {
-      literal =
-        Expr(AssignExpr
-             (ColEq,
-              (Var "b"),
-              (RefBrack ((Var "a"), (Value (String "English")))))
+                (Value (String "French"), Value (String "Salut"))
+              ])));
+        with_mods = []
+      };
+      {
+        literal
+        =
+        Expr (AssignExpr (ColEq, (Var "b"), (RefBrack ((Var "a"), (Value (String "English"))))));
+        with_mods = []
+      };
+      {
+        literal
+        =
+        Expr (AssignExpr (ColEq, (Var "c"), (Ast.Array [Value (Number 41); Value (Number 47)])));
+        with_mods = []
+      };
+      {
+        literal = Expr (AssignExpr (ColEq, (Var "d"), (Ast.Array [Var "a"; Var "c"])));
+        with_mods = []
+      };
+      {
+        literal
+        =
+        Expr (AssignExpr (ColEq, (Var "e"), (RefBrack (RefBrack (Var "d", Var "f"), (Var "g")))));
+        with_mods = []
+      };
+      { literal = ArrayComprOutput (Ast.Array [Var "e"; Var "f"; Var "g"]); with_mods = [] }
+    ]
+  }
 
-        );
-      with_mods=[];
-    };
-    {
-      literal =
-        Expr(AssignExpr
-             (ColEq,
-              (Var "c"),
-              (Ast.Array [Value (Number 41); Value (Number 47)]))
+let intr2 = Interpreter.make_new ()
 
-        );
-      with_mods=[];
-    };
-    {
-      literal =
-        Expr(AssignExpr
-             (ColEq,
-              (Var "d"),
-              (Ast.Array [Var "a"; Var "c"]))
+let v6, intr3 = Interpreter.eval_user_query intr2 query
 
-        );
-      with_mods=[];
-    };
-    {
-      literal =
-        Expr(AssignExpr
-             (ColEq,
-              (Var "e"),
-              (RefBrack (RefBrack (Var "d", Var "f"), (Var "g"))))
+let query1 =
+  { stmts = List.Tot.append query.stmts [{ literal = Expr (Value (Bool false)); with_mods = [] }] }
 
-        );
-      with_mods=[];
-    };
-    { literal = ArrayComprOutput (Ast.Array [Var "e"; Var "f"; Var "g"]);
-      with_mods = [];
-    }
-  ];
-}
+let intr4 = Interpreter.make_new ()
 
-let intr2 = Interpreter.make_new()
-let (v6, intr3) = Interpreter.eval_user_query intr2 query
-
-let query1 = {
-  stmts = List.Tot.append query.stmts
-  [{
-    literal = Expr(Value (Bool false)); with_mods=[];
-  }]
-}
-
-let intr4 = Interpreter.make_new()
-let (v7, intr5) = Interpreter.eval_user_query intr4 query1
-
+let v7, intr5 = Interpreter.eval_user_query intr4 query1
 
 let main () =
   FStar.IO.print_string (to_json_pretty v1);
@@ -134,7 +126,12 @@ let main () =
   FStar.IO.print_string (to_json_pretty v7);
   FStar.IO.print_string "\n"
 
+
+
 //Run ``main ()`` when the module loads
+
 #push-options "--warn_error -272"
+
 let _ = main ()
+
 #pop-options
