Rego.Value.fst
@@ -2,221 +2,211 @@
 // Licensed under the MIT License.
 
 module Rego.Value
+
 open FStar.String
 
-  let rec array_cmp (l1:list value) (l2:list value) : Tot ord (decreases l1)=
-    match l1, l2 with
-      | hd1::tl1, hd2::tl2  ->
-        (match cmp hd1 hd2 with
-          | 0 -> array_cmp tl1 tl2
+let rec array_cmp (l1 l2: list value) : Tot ord (decreases l1) =
+  match l1, l2 with
+  | hd1 :: tl1, hd2 :: tl2 ->
+    (match cmp hd1 hd2 with
+      | 0 -> array_cmp tl1 tl2
+      | r -> r)
+  | [], [] -> 0
+  | _, [] -> 1
+  | [], _ -> - 1
+
+and object_cmp (l1 l2: list (value * value)) : Tot ord (decreases l1) =
+  match l1, l2 with
+  | (k1, v1) :: tl1, (k2, v2) :: tl2 ->
+    (match cmp k1 k2 with
+      | 0 ->
+        (match cmp v1 v2 with
+          | 0 -> object_cmp tl1 tl2
           | r -> r)
-      | [], [] -> 0
-      | _ , [] -> 1
-      | [], _ -> -1
+      | r -> r)
+  | [], [] -> 0
+  | _, [] -> 1
+  | [], _ -> - 1
 
-  and object_cmp (l1: list (value * value)) (l2 : list (value*value)) : Tot ord (decreases l1) =
-    match l1, l2 with
-      | (k1, v1)::tl1, (k2, v2)::tl2 ->
-        (match cmp k1 k2 with
-          | 0 ->
-            (match cmp v1 v2 with
-              | 0 -> object_cmp tl1 tl2
-              | r -> r)
-          | r -> r)
-      | [], [] -> 0
-      | _ , [] -> 1
-      | [], _ -> -1
+and cmp (v1 v2: value) : ord =
+  match v1, v2 with
+  | Null, Null -> 0
+  | Null, _ -> - 1 (* Null is lesser than other values *)
+  | _, Null -> 1
+  | Bool b1, Bool b2 ->
+    (match b1, b2 with
+      | false, false -> 0
+      | false, _ -> - 1
+      | true, true -> 0
+      | true, _ -> 1)
+  | Bool _, _ -> - 1 (* Bool is greater than Null *)
+  | _, Bool _ -> 1
+  | Number n1, Number n2 -> if n1 > n2 then 1 else if n1 = n2 then 0 else - 1
+  | Number _, _ -> - 1 (* Numner is greater than Bool *)
+  | _, Number _ -> 1
+  | String s1, String s2 ->
+    (match String.compare s1 s2 with
+      | 1 -> 1
+      | 0 -> 0
+      | _ -> - 1)
+  | String _, _ -> - 1 (* String is greater than Number *)
+  | _, String _ -> 1
+  | Array a1, Array a2 -> array_cmp a1 a2
+  | Array _, _ -> - 1 (* Array is greater than String *)
+  | _, Array _ -> 1
+  | Set s1, Set s2 -> array_cmp s1 s2
+  | Set _, _ -> - 1 (* Set is greater than Array *)
+  | _, Set _ -> 1
+  | Object o1, Object o2 -> object_cmp o1 o2
+  | Object _, Undefined -> - 1 (* Object is greater than Set *)
+  | Undefined, Object _ -> 1
+  | Undefined, Undefined -> 0
 
-  and cmp (v1:value) (v2:value) : ord =
-    match v1, v2 with
-      | Null, Null -> 0
-      | Null, _ -> -1  (* Null is lesser than other values *)
-      | _, Null -> 1
+let insert_into_array (arr v: value) : value =
+  match arr with
+  | Array a -> Array (List.Tot.append a [v])
+  | _ -> Undefined
 
-      | Bool b1, Bool b2 ->
-        (match b1, b2 with
-          | false, false -> 0
-          | false, _ -> -1
-          | true, true -> 0
-          | true, _ -> 1)
-      | Bool _, _ -> -1  (* Bool is greater than Null *)
-      | _, Bool _ -> 1
+let rec insert_into_fields (fields: list (value * value)) (key value: value) =
+  match fields with
+  | (k, v) :: tl ->
+    (match cmp k key with
+      | 0 -> (key, value) :: tl
+      | 1 -> (key, value) :: (k, v) :: tl
+      | -1 -> (k, v) :: insert_into_fields tl key value)
+  | _ -> [(key, value)]
 
+let insert_into_object (obj key value: value) =
+  match obj with
+  | Object fields -> Object (insert_into_fields fields key value)
+  | _ -> Undefined
 
-      | Number n1, Number n2 ->
-        if n1 > n2 then 1 else if n1 = n2 then 0 else -1
-      | Number _, _ -> -1  (* Numner is greater than Bool *)
-      | _, Number _ -> 1
+let rec insert_into_set_items (items: list value) (item: value) =
+  match items with
+  | v :: tl ->
+    (match cmp v item with
+      | 0 -> v :: tl
+      | 1 -> item :: v :: tl
+      | -1 -> v :: insert_into_set_items tl item)
+  | _ -> [item]
 
-      | String s1, String s2 ->
-        (match String.compare s1 s2 with
-          | 1 -> 1
-          | 0 -> 0
-          | _ -> -1)
-      | String _, _ -> -1  (* String is greater than Number *)
-      | _, String _ -> 1
+let insert_into_set (set item: value) : value =
+  match set with
+  | Set items -> Set (insert_into_set_items items item)
+  | _ -> Undefined
 
-      | Array a1, Array a2 -> array_cmp a1 a2
-      | Array _, _ -> -1  (* Array is greater than String *)
-      | _, Array _ -> 1
+let rec lookup_field (fields: list (value * value)) (key: value) : value =
+  match fields with
+  | (k, v) :: tl -> (if (cmp k key) = 0 then v else lookup_field tl key)
+  | _ -> Undefined
 
-      | Set s1, Set s2 -> array_cmp s1 s2
-      | Set _, _ -> -1   (* Set is greater than Array *)
-      | _, Set _ -> 1
+let rec lookup_path (obj: value) (path: list value) : Tot value (decreases (List.length path)) =
+  match obj, path with
+  | Undefined, _ -> Undefined
+  | _, [] -> obj
+  | Object fields, field :: tl ->
+    (match lookup_field fields field with
+      | Undefined -> Undefined
+      | obj -> lookup_path obj tl)
+  | _ -> Undefined
 
-      | Object o1, Object o2 -> object_cmp o1 o2
-      | Object _, Undefined -> -1 (* Object is greater than Set *)
-      | Undefined, Object _ -> 1
+let rec insert_at_path (obj: value) (path: list value) (v: value)
+    : Tot value (decreases (List.length path)) =
+  match obj, path with
+  | Object _, p :: [] -> insert_into_object obj p v
+  | Object _, p :: tl ->
+    (match lookup_path obj ([p]) with
+      | Undefined ->
+        (* The key p does not exist in obj *)
+        let subobj = insert_at_path (Object []) tl v (* create subobject *) in
+        (* insert subobj as field p into obj *)
+        insert_into_object obj p subobj
+      | subobj ->
+        (* The key p exists in obj *)
+        let subobj1 = insert_at_path subobj tl v (* insert v at path tl into subobj *) in
+        (match subobj1 with
+          | Undefined -> Undefined (* insertion failed *)
+          | _ ->
+            (* insertion succeeded. Insert subobj as field p in obj *)
+            insert_into_object obj p subobj))
+  | _ ->
+    (* not an object or invalid path *)
+    Undefined
 
-      | Undefined, Undefined -> 0
+let escape_char (c: FStar.Char.char) : list char =
+  match c with
+  | '\n' -> ['\\'; 'n']
+  | '\r' -> ['\\'; 'r']
+  | '\t' -> ['\\'; 't']
+  | '"' -> ['\\'; '"']
+  | _ -> [c]
 
-  let insert_into_array (arr:value) (v:value) : value =
-    match arr with
-    | Array a -> Array (List.Tot.append a [v])
-    | _ -> Undefined
-  
-  let rec insert_into_fields (fields:list (value*value)) (key:value) (value:value) =
-      match fields with
-        | (k, v)::tl ->
-          (match cmp k key with
-            | 0 -> (key, value)::tl
-            | 1 -> (key,value)::(k, v)::tl
-            | -1 -> (k,v)::insert_into_fields tl key value)
-        | _ -> (key, value)::[]
+let escaped (s: string) : Tot string =
+  String.string_of_list (List.Tot.collect escape_char (String.list_of_string s))
 
-  let insert_into_object (obj:value) (key:value) (value:value)  =
-    match obj with
-      | Object fields -> Object (insert_into_fields fields key value)
-      | _ -> Undefined
+let rec array_elem_to_json (a: list value) : Tot (list string) (decreases a) =
+  match a with
+  | [] -> []
+  | hd :: tl -> to_json hd :: array_elem_to_json tl
 
-  let rec insert_into_set_items (items:list value) (item:value) =
-      match items with
-        | v::tl ->
-          (match cmp v item with
-            | 0 -> v::tl
-            | 1 -> item::v::tl
-            | -1 -> v::insert_into_set_items tl item)
-        | _ -> item::[]
+and field_to_json (a: list (value * value)) : Tot (list string) (decreases a) =
+  match a with
+  | [] -> []
+  | (k, v) :: tl ->
+    let k_json =
+      match k with
+      | String s -> Printf.sprintf "\"%s\"" (escaped s)
+      | _ -> Printf.sprintf "\"%s\"" (escaped (to_json k))
+    in
+    let v_json = to_json v in
+    (Printf.sprintf "%s: %s" k_json v_json) :: field_to_json tl
 
-   let insert_into_set (set:value) (item:value) : value =
-       match set with
-       | Set items -> Set (insert_into_set_items items item)
-       | _ -> Undefined
+and to_json (v: value) : Tot string (decreases v) =
+  match v with
+  | Null -> "null"
+  | Bool b -> string_of_bool b
+  | Number n -> string_of_int n
+  | String s -> Printf.sprintf "\"%s\"" s
+  | Array a
+  | Set a ->
+    let elems_json = array_elem_to_json a in
+    Printf.sprintf "[%s]" (String.concat "," elems_json)
+  | Object fields ->
+    let flds_json = field_to_json fields in
+    Printf.sprintf "{%s}" (String.concat "," flds_json)
+  | Undefined -> "<undefined>"
 
+let rec array_elem_to_json_p (a: list value) (indent: string) : Tot (list string) (decreases a) =
+  match a with
+  | [] -> []
+  | hd :: tl -> to_json_p_impl hd indent :: array_elem_to_json_p tl indent
 
-   let rec lookup_field (fields: list (value*value)) (key:value) : value=
-       match fields with
-       	| (k,v)::tl -> (if (cmp k key) = 0 then v else lookup_field tl key)
-	| _ -> Undefined
+and field_to_json_p (a: list (value * value)) (indent: string) : Tot (list string) (decreases a) =
+  match a with
+  | [] -> []
+  | (k, v) :: tl ->
+    let k_json =
+      match k with
+      | String s -> Printf.sprintf "%s\"%s\"" indent (escaped s)
+      | _ -> Printf.sprintf "%s\"%s\"" indent (escaped (to_json k))
+    in
+    let v_json = to_json_p_impl v indent in
+    (Printf.sprintf "%s: %s" k_json v_json) :: field_to_json_p tl indent
 
-   let rec lookup_path (obj:value) (path:list value)
-       : Tot value (decreases (List.length path))
-       =
-       match obj, path with
-        | Undefined, _ -> Undefined
-        | _, [] -> obj
-	| Object fields, (field::tl) ->
-	  (match lookup_field fields field with
-	  | Undefined -> Undefined
-	  | obj -> lookup_path obj tl)
-	| _ -> Undefined
+and to_json_p_impl (v: value) (indent: string) : Tot string (decreases v) =
+  match v with
+  | Null -> "null"
+  | Bool b -> string_of_bool b
+  | Number n -> string_of_int n
+  | String s -> Printf.sprintf "\"%s\"" s
+  | Array a
+  | Set a ->
+    let indent' = indent ^ "  " in
+    let elems_json = array_elem_to_json_p a indent' in
+    Printf.sprintf "[\n%s%s\n%s]" indent' (String.concat (",\n" ^ indent') elems_json) indent
+  | Object fields ->
+    let flds_json = field_to_json_p fields (indent ^ "  ") in
+    Printf.sprintf "{\n%s\n%s}" (String.concat ",\n" flds_json) indent
+  | Undefined -> "<undefined>"
 
-   let rec insert_at_path (obj:value) (path:list value)(v:value)
-       : Tot value (decreases (List.length path))
-       =
-       match obj, path with
-         | Object _, p::[] -> insert_into_object obj p v
-         | Object _, p::tl ->
-           (match lookup_path obj (p::[]) with
-             (* The key p does not exist in obj *)
-             | Undefined ->
-               (* create subobject *)
-               let subobj = insert_at_path (Object []) tl v in
-                 (* insert subobj as field p into obj *)
-                 insert_into_object obj p subobj
-
-             (* The key p exists in obj *)
-             | subobj ->
-               (* insert v at path tl into subobj *)
-               let subobj1 = insert_at_path subobj tl v in
-                 (match subobj1 with
-                   (* insertion failed *)
-                   | Undefined -> Undefined
-                   (* insertion succeeded. Insert subobj as field p in obj *)
-                   | _ -> insert_into_object obj p subobj))
-
-         (* not an object or invalid path *)
-         | _  -> Undefined
-
-
-  let escape_char (c:FStar.Char.char) : list char =
-    match c with
-    | '\n' -> '\\'::'n'::[]
-    | '\r' -> '\\'::'r'::[]
-    | '\t' -> '\\'::'t'::[]
-    | '"' -> '\\'::'"'::[]
-    | _ -> c::[]
-
-  let escaped (s:string) : Tot string =
-    String.string_of_list (List.Tot.collect escape_char (String.list_of_string s))
-
-  let rec array_elem_to_json (a:list value) : Tot (list string) (decreases a) =
-    match a with
-    | [] -> []
-    | hd::tl -> to_json hd::array_elem_to_json tl
-
-  and field_to_json (a:list (value*value)) : Tot (list string) (decreases a) =
-    match a with
-    | [] -> []
-    | (k, v)::tl ->
-      let k_json = match k with
-        | String s -> Printf.sprintf "\"%s\"" (escaped s)
-        | _ -> Printf.sprintf "\"%s\"" (escaped (to_json k)) in
-      let v_json = to_json v in
-      (Printf.sprintf "%s: %s" k_json v_json)::field_to_json tl
-
-  and to_json (v:value) : Tot string (decreases v)  =
-    match v with
-    | Null -> "null"
-    | Bool b -> string_of_bool b
-    | Number n -> string_of_int n
-    | String s -> Printf.sprintf "\"%s\"" s
-    | Array a | Set a ->
-      let elems_json = array_elem_to_json a in
-      Printf.sprintf "[%s]" (String.concat "," elems_json)
-    | Object fields ->
-      let flds_json = field_to_json fields in
-      Printf.sprintf "{%s}" (String.concat "," flds_json)
-    | Undefined -> "<undefined>"
-
-  let rec array_elem_to_json_p (a:list value) (indent:string) : Tot (list string) (decreases a) =
-    match a with
-    | [] -> []
-    | hd::tl -> to_json_p_impl hd indent::array_elem_to_json_p tl indent
-
-  and field_to_json_p (a:list (value*value)) (indent:string) : Tot (list string) (decreases a) =
-    match a with
-    | [] -> []
-    | (k, v)::tl ->
-      let k_json = match k with
-        | String s -> Printf.sprintf "%s\"%s\"" indent (escaped s)
-        | _ -> Printf.sprintf "%s\"%s\"" indent (escaped (to_json k)) in
-      let v_json = to_json_p_impl v indent in
-      (Printf.sprintf "%s: %s" k_json v_json)::field_to_json_p tl indent
-
-  and to_json_p_impl (v:value) (indent:string) : Tot string (decreases v)  =
-    match v with
-    | Null -> "null"
-    | Bool b -> string_of_bool b
-    | Number n -> string_of_int n
-    | String s -> Printf.sprintf "\"%s\"" s
-    | Array a | Set a ->
-      let indent' = indent ^ "  " in
-      let elems_json = array_elem_to_json_p a indent' in
-      Printf.sprintf "[\n%s%s\n%s]" indent' (String.concat (",\n" ^ indent') elems_json) indent
-    | Object fields ->
-      let flds_json = field_to_json_p fields (indent ^ "  ") in
-      Printf.sprintf "{\n%s\n%s}" (String.concat ",\n" flds_json) indent
-    | Undefined -> "<undefined>"
-
-  let to_json_pretty (v:value) : string = to_json_p_impl  v ""
+let to_json_pretty (v: value) : string = to_json_p_impl v ""
