Rego.Ast.fsti
@@ -3,111 +3,91 @@
 
 module Rego.Ast
 
-  #push-options "--warn_error -331"
-  type binOp =
-    | And
-    | Or
+#push-options "--warn_error -331"
 
-  and  arithOp =
-    | Add
-    | Sub
-    | Mul
-    | Divv
-    | Mod
-
-  and boolOp =
-    | Lt
-    | Le
-    | Eq
-    | Ge
-    | Gt
-    | Ne
-
-  and assignOp =
-    | EqAssign  (* Changed name to differentiate from Assign in boolOp *)
-    | ColEq
-
-
-  and ident = string
-
+type binOp =
+  | And
+  | Or
+and arithOp =
+  | Add
+  | Sub
+  | Mul
+  | Divv
+  | Mod
+and boolOp =
+  | Lt
+  | Le
+  | Eq
+  | Ge
+  | Gt
+  | Ne
+and assignOp =
+  | EqAssign (* Changed name to differentiate from Assign in boolOp *)
+  | ColEq
+and ident = string
+and expr : eqtype =
   (* without eqtype annotation "Failed to solve universe inequalities for inductives" *)
-  and expr:eqtype = 
-    | Value of Rego.Value.value
-    | Var of ident
-    | Array of (items:list expr)
-    | Set of (items:list expr)
-    | Object of (fields:list (expr * expr))
-    | ArrayCompr of query
-    | SetCompr of query
-    | ObjectCompr of query
-    | Call of (fcn:expr) * (params:list expr)
-    | UnaryExpr of expr
-    | RefDot of (refr:expr) * (field:string)
-    | RefBrack of (refr:expr) * (index:expr)
-    | BinExpr of binOp * (lhs:expr) * (rhs:expr)
-    | BoolExpr of boolOp * (lhs:expr) * (rhs:expr)
-    | ArithExpr of arithOp * (lhs:expr) * (rhs:expr)
-    | AssignExpr of assignOp * (lhs:expr) * (rhs:expr)
-    | MembershipExpr of (key:expr) * (value:expr) * (collection:expr)
+  | Value of Rego.Value.value
+  | Var of ident
+  | Array of (items : list expr)
+  | Set of (items : list expr)
+  | Object of (fields : list (expr * expr))
+  | ArrayCompr of query
+  | SetCompr of query
+  | ObjectCompr of query
+  | Call of (fcn : expr) * (params : list expr)
+  | UnaryExpr of expr
+  | RefDot of (refr : expr) * (field : string)
+  | RefBrack of (refr : expr) * (index : expr)
+  | BinExpr of binOp * (lhs : expr) * (rhs : expr)
+  | BoolExpr of boolOp * (lhs : expr) * (rhs : expr)
+  | ArithExpr of arithOp * (lhs : expr) * (rhs : expr)
+  | AssignExpr of assignOp * (lhs : expr) * (rhs : expr)
+  | MembershipExpr of (key : expr) * (value : expr) * (collection : expr)
+and literal =
+  | SomeVars of (var : list ident)
+  | SomeIn of (key : option expr) * (value : expr) * (collection : expr)
+  | Expr of expr
+  | NotExpr of (a : expr)
+  | Every of (key : option ident) * (value : ident) * (domain : expr) * query
+  | ArrayComprOutput of (e : expr)
+  | SetComprOutput of (e : expr)
+  | ObjectComprOutput of (k : expr) * (v : expr)
+  | LoopExpr of expr
+and withModifier = {
+  refr:expr;
+  as_:expr
+}
+and literalStmt = {
+  literal:literal;
+  with_mods:list withModifier
+}
+and query = { stmts:list literalStmt }
+and ruleAssign = {
+  op:assignOp;
+  value:expr
+}
+and ruleBody = {
+  assign:option ruleAssign;
+  query:query
+}
+and ruleHead =
+  | Compr of (refr : expr) * (assign : option ruleAssign)
+  | Set_ of (refr : expr) * (key : option expr)
+  | Func of (refr : expr) * (args : list expr) * (assign : option ruleAssign)
+and rule =
+  | Spec of (head : ruleHead) * (bodies : list ruleBody)
+  | Default of (refr : expr) * (args : list expr) * (op : assignOp) * (value : expr)
+and package = { refr:expr }
+and import = {
+  refr:expr;
+  as_:option ident
+}
+and regoModule = {
+  package:package;
+  imports:list import;
+  policy:list rule;
+  rego_v1:bool
+}
 
-  and literal =
-    | SomeVars of (var:list ident)
-    | SomeIn of (key:option expr) * (value:expr) * (collection:expr)
-    | Expr of expr
-    | NotExpr of (a:expr)
-    | Every of (key:option ident) * (value:ident) * (domain:expr) * query
-    | ArrayComprOutput of (e:expr)
-    | SetComprOutput of (e:expr)
-    | ObjectComprOutput of (k:expr) * (v:expr)
-    | LoopExpr of expr
-
-  and withModifier =  {
-      refr: expr;
-      as_: expr;
-  }
-
-  and literalStmt = {
-      literal: literal;
-      with_mods: list withModifier;
-  }
-
-  and query = {
-    stmts: list literalStmt
-  }
-
-  and ruleAssign = {
-    op: assignOp;
-    value: expr;
-  }
-
-  and ruleBody = {
-    assign: option ruleAssign;
-    query: query;
-  }
-
-  and ruleHead =
-    | Compr of (refr:expr) * (assign: option ruleAssign)
-    | Set_ of (refr:expr) * (key:option expr)
-    | Func of (refr:expr) * (args:list expr) * (assign: option ruleAssign)
-
-  and rule =
-    | Spec of (head:ruleHead) * (bodies: list ruleBody)
-    | Default of (refr:expr) * (args:list expr) * (op:assignOp) * (value:expr)
-
-  and package = {
-    refr: expr;
-  }
-
-  and import = {
-    refr: expr;
-    as_: option ident;
-  }
-
-  and regoModule = {
-    package: package;
-    imports: list import;
-    policy: list rule;
-    rego_v1: bool;
-  }
-
- #pop-options
+#pop-options
