Rego.Value.fsti
@@ -3,30 +3,31 @@
 
 module Rego.Value
 
-  [@@ PpxDerivingYoJson; PpxDerivingShow ]
-  type value:eqtype =
-    | Null
-    | Bool of bool
-    | Number of int (* TODO: number can be i64, u64, f64 or big decimal *)
-    | String of string
-    | Array of list value
-    | Set of list value
-    | Object of list (value * value)
-    | Undefined
+[@@ PpxDerivingYoJson; PpxDerivingShow]
+type value : eqtype =
+  | Null
+  | Bool of bool
+  | Number of int (* TODO: number can be i64, u64, f64 or big decimal *)
+  | String of string
+  | Array of list value
+  | Set of list value
+  | Object of list (value * value)
+  | Undefined
 
-  type ord = x:int { x = -1 || x = 0 || x = 1}
-  
-  val cmp (v1:value) (v2:value) : ord
+type ord = x: int{x = - 1 || x = 0 || x = 1}
 
-  val insert_into_array (arr:value) (v:value) : value
-  
-  val insert_into_object (obj:value) (key:value) (v:value) : value
+val cmp (v1 v2: value) : ord
 
-  val insert_into_set (set:value) (item:value) : value
+val insert_into_array (arr v: value) : value
 
-  val lookup_path (obj:value) (path:list value) : value
+val insert_into_object (obj key v: value) : value
 
-  val insert_at_path (obj:value) (path: list value) (v:value) : value
+val insert_into_set (set item: value) : value
 
-  val to_json (v:value) : string 
-  val to_json_pretty (v:value) : string
+val lookup_path (obj: value) (path: list value) : value
+
+val insert_at_path (obj: value) (path: list value) (v: value) : value
+
+val to_json (v: value) : string
+
+val to_json_pretty (v: value) : string
